fixed most of the compilation warnings; need to compute Brzozowski's upper bound to fix the last one

ExampleLexer.v
@@ -399,9 +399,10 @@ Definition ru_rbrace := (toS "RIGHT_BRACE", regex_rbrace).
 (*** Compile rules and export ***)
 Definition rus : list Rule := [ru_ws;ru_number;ru_string;ru_true;ru_false;ru_null;ru_colon;ru_comma;ru_lbrack;ru_rbrack;ru_lbrace;ru_rbrace].
 
-Definition lex := lex__M.
-Definition lex' := lex'__M.
+Definition lex := lex_M.
+Definition lex' := lex'_M.
 
+Set Warnings "-extraction-opaque-accessed,-extraction".
 Extraction "Evaluation/instance.ml" lex rus.
 
 
